Add small-step semantics for boolean expressions with rules and steps

ExprEval/Basic.lean
@@ -18,7 +18,7 @@ def eval (val: V -> Int) (e: ArExpr V) : Int :=
         | ArExpr.Mul lhs rhs => (eval val lhs) * (eval val rhs)
         | ArExpr.Var v => val v
 
--- My small steps semantic
+-- Small steps semantic for arithmetic expressions
 
 inductive ArStep: (val: V -> Int) -> (ArExpr V) -> (ArExpr V) -> Prop where
     | getVarValue (var: V) :
@@ -26,31 +26,31 @@ inductive ArStep: (val: V -> Int) -> (ArExpr V) -> (ArExpr V) -> Prop where
             val
             (ArExpr.Var var)
             (ArExpr.Const (val var))
-    | addConstConst(n1 n2: Int) :
+    | addConstConst(n₁ n₂: Int) :
         ArStep
             val
-            (ArExpr.Add (ArExpr.Const n1) (ArExpr.Const n2))
-            (ArExpr.Const (n1 + n2))
-    | subConstConst(n1 n2: Int) :
+            (ArExpr.Add (ArExpr.Const n₁) (ArExpr.Const n₂))
+            (ArExpr.Const (n₁ + n₂))
+    | subConstConst(n₁ n₂: Int) :
         ArStep
             val
-            (ArExpr.Sub (ArExpr.Const n1) (ArExpr.Const n2))
-            (ArExpr.Const (n1 - n2))
-    | mulConstConst(n1 n2: Int) :
+            (ArExpr.Sub (ArExpr.Const n₁) (ArExpr.Const n₂))
+            (ArExpr.Const (n₁ - n₂))
+    | mulConstConst(n₁ n₂: Int) :
         ArStep
             val
-            (ArExpr.Mul (ArExpr.Const n1) (ArExpr.Const n2))
-            (ArExpr.Const (n1 * n2))
-    | addLeft (e1 e1' e2) : ArStep val e1 e1' -> ArStep val (ArExpr.Add e1 e2) (ArExpr.Add e1' e2)
+            (ArExpr.Mul (ArExpr.Const n₁) (ArExpr.Const n₂))
+            (ArExpr.Const (n₁ * n₂))
+    | addLeft (e₁ e₁' e₂) : ArStep val e₁ e₁' -> ArStep val (ArExpr.Add e₁ e₂) (ArExpr.Add e₁' e₂)
 
-    | subLeft (e1 e1' e2) : ArStep val e1 e1' -> ArStep val (ArExpr.Sub e1 e2) (ArExpr.Sub e1' e2)
+    | subLeft (e₁ e₁' e₂) : ArStep val e₁ e₁' -> ArStep val (ArExpr.Sub e₁ e₂) (ArExpr.Sub e₁' e₂)
 
-    | mulLeft (e1 e1' e2) : ArStep val e1 e1' -> ArStep val (ArExpr.Mul e1 e2) (ArExpr.Mul e1' e2)
+    | mulLeft (e₁ e₁' e₂) : ArStep val e₁ e₁' -> ArStep val (ArExpr.Mul e₁ e₂) (ArExpr.Mul e₁' e₂)
 
-    | addRight (n: Int) (e2 e2': ArExpr V) : ArStep val e2 e2' -> ArStep val (ArExpr.Add (ArExpr.Const n) e2)  (ArExpr.Add (ArExpr.Const n) e2')
+    | addRight (n: Int) (e₂ e₂': ArExpr V) : ArStep val e₂ e₂' -> ArStep val (ArExpr.Add (ArExpr.Const n) e₂)  (ArExpr.Add (ArExpr.Const n) e₂')
 
-    | subRight (n: Int) (e2 e2': ArExpr V) : ArStep val e2 e2' -> ArStep val (ArExpr.Sub (ArExpr.Const n) e2)  (ArExpr.Sub (ArExpr.Const n) e2')
-    | mulRight (n: Int) (e2 e2': ArExpr V) : ArStep val e2 e2' -> ArStep val (ArExpr.Mul (ArExpr.Const n) e2)  (ArExpr.Mul (ArExpr.Const n) e2')
+    | subRight (n: Int) (e₂ e₂': ArExpr V) : ArStep val e₂ e₂' -> ArStep val (ArExpr.Sub (ArExpr.Const n) e₂)  (ArExpr.Sub (ArExpr.Const n) e₂')
+    | mulRight (n: Int) (e₂ e₂': ArExpr V) : ArStep val e₂ e₂' -> ArStep val (ArExpr.Mul (ArExpr.Const n) e₂)  (ArExpr.Mul (ArExpr.Const n) e₂')
 
 inductive ArStepStar : (val: V -> Int) -> (ArExpr V) -> (ArExpr V) -> Prop where
     | refl val e : ArStepStar val e e
@@ -60,17 +60,17 @@ theorem arstep_preserve_eval (e e': ArExpr V): (ArStep V val) e e' -> eval V val
     intro h
     induction h with
 
-    | addConstConst n1 n2
-    | subConstConst n1 n2
-    | mulConstConst n1 n2 => simp [eval]
+    | addConstConst n₁ n₂
+    | subConstConst n₁ n₂
+    | mulConstConst n₁ n₂ => simp [eval]
 
-    | addLeft e1 e1' e2 _ ih
-    | subLeft e1 e1' e2 _ ih
-    | mulLeft e1 e1' e2 _ ih => simp [eval, ih]
+    | addLeft e₁ e₁' e₂ _ ih
+    | subLeft e₁ e₁' e₂ _ ih
+    | mulLeft e₁ e₁' e₂ _ ih => simp [eval, ih]
 
-    | addRight n e2 e1' _ ih
-    | subRight n e2 e1' _ ih
-    | mulRight n e2 e1' _ ih => simp [eval, ih]
+    | addRight n e₂ e₁' _ ih
+    | subRight n e₂ e₁' _ ih
+    | mulRight n e₂ e₁' _ ih => simp [eval, ih]
 
     | getVarValue var => simp [eval]
 
@@ -82,8 +82,8 @@ theorem arstepstar_preserves_eval (e e': ArExpr V) :
     | refl _ => rfl
     | trans _ _ _ h1 _ ih => rw [arstep_preserve_eval _ _ _ h1, ih]
 
-theorem arstepstar_add_left (e1 e1' e2: ArExpr V) :
-    ArStepStar V val e1 e1' -> ArStepStar V val (ArExpr.Add e1 e2) (ArExpr.Add e1' e2) := by
+theorem arstepstar_add_left (e₁ e₁' e₂: ArExpr V) :
+    ArStepStar V val e₁ e₁' -> ArStepStar V val (ArExpr.Add e₁ e₂) (ArExpr.Add e₁' e₂) := by
     intro h
     induction h with
     | refl _ => apply ArStepStar.refl
@@ -92,26 +92,26 @@ theorem arstepstar_add_left (e1 e1' e2: ArExpr V) :
         . exact ArStep.addLeft _ _ _ step
         . exact ih
 
-theorem arstepstar_add_right (n: Int) (e2 e2': ArExpr V) :
-    ArStepStar V val e2 e2' ->
+theorem arstepstar_add_right (n: Int) (e₂ e₂': ArExpr V) :
+    ArStepStar V val e₂ e₂' ->
         ArStepStar V val
-            (ArExpr.Add (ArExpr.Const n) e2)
-            (ArExpr.Add (ArExpr.Const n) e2') := by
+            (ArExpr.Add (ArExpr.Const n) e₂)
+            (ArExpr.Add (ArExpr.Const n) e₂') := by
     intro h
     induction h with
     | refl _ => apply ArStepStar.refl
-    | trans e1 e2 e3 step1 step2 ih =>
+    | trans e₁ e₂ e3 step1 step2 ih =>
         apply ArStepStar.trans
         . apply ArStep.addRight _ _ _ step1
         . exact ih
 
 
 
-theorem arstepstar_sub_left (e1 e1' e2: ArExpr V) :
-    ArStepStar V val e1 e1' ->
+theorem arstepstar_sub_left (e₁ e₁' e₂: ArExpr V) :
+    ArStepStar V val e₁ e₁' ->
         ArStepStar V val
-            (ArExpr.Sub e1 e2)
-            (ArExpr.Sub e1' e2) := by
+            (ArExpr.Sub e₁ e₂)
+            (ArExpr.Sub e₁' e₂) := by
     intro h
     induction h with
     | refl _ => apply ArStepStar.refl
@@ -120,26 +120,26 @@ theorem arstepstar_sub_left (e1 e1' e2: ArExpr V) :
         . exact ArStep.subLeft _ _ _ step
         . exact ih
 
-theorem arstepstar_sub_right (n: Int) (e2 e2': ArExpr V) :
-    ArStepStar V val e2 e2' ->
+theorem arstepstar_sub_right (n: Int) (e₂ e₂': ArExpr V) :
+    ArStepStar V val e₂ e₂' ->
         ArStepStar V val
-            (ArExpr.Sub (ArExpr.Const n) e2)
-            (ArExpr.Sub (ArExpr.Const n) e2') := by
+            (ArExpr.Sub (ArExpr.Const n) e₂)
+            (ArExpr.Sub (ArExpr.Const n) e₂') := by
     intro h
     induction h with
     | refl _ => apply ArStepStar.refl
-    | trans e1 e2 e3 step1 step2 ih =>
+    | trans e₁ e₂ e3 step1 step2 ih =>
         apply ArStepStar.trans
         . apply ArStep.subRight _ _ _ step1
         . exact ih
 
 
 
-theorem arstepstar_mul_left (e1 e1' e2: ArExpr V) :
-    ArStepStar V val e1 e1' ->
+theorem arstepstar_mul_left (e₁ e₁' e₂: ArExpr V) :
+    ArStepStar V val e₁ e₁' ->
         ArStepStar V val
-            (ArExpr.Mul e1 e2)
-            (ArExpr.Mul e1' e2) := by
+            (ArExpr.Mul e₁ e₂)
+            (ArExpr.Mul e₁' e₂) := by
     intro h
     induction h with
     | refl _ => apply ArStepStar.refl
@@ -148,23 +148,23 @@ theorem arstepstar_mul_left (e1 e1' e2: ArExpr V) :
         . exact ArStep.mulLeft _ _ _ step
         . exact ih
 
-theorem arstepstar_mul_right (n: Int) (e2 e2': ArExpr V) :
-    ArStepStar V val e2 e2' ->
+theorem arstepstar_mul_right (n: Int) (e₂ e₂': ArExpr V) :
+    ArStepStar V val e₂ e₂' ->
         ArStepStar V val
-            (ArExpr.Mul (ArExpr.Const n) e2)
-            (ArExpr.Mul (ArExpr.Const n) e2') := by
+            (ArExpr.Mul (ArExpr.Const n) e₂)
+            (ArExpr.Mul (ArExpr.Const n) e₂') := by
     intro h
     induction h with
     | refl _ => apply ArStepStar.refl
-    | trans e1 e2 e3 step1 step2 ih =>
+    | trans e₁ e₂ e3 step1 step2 ih =>
         apply ArStepStar.trans
         . apply ArStep.mulRight _ _ _ step1
         . exact ih
 
-theorem chasles_step_star {e1 e2 e3: ArExpr V}:
-    ArStepStar V val e1 e2 ->
-        ArStepStar V val e2 e3 ->
-            ArStepStar V val e1 e3 := by
+theorem chasles_step_star {e₁ e₂ e3: ArExpr V}:
+    ArStepStar V val e₁ e₂ ->
+        ArStepStar V val e₂ e3 ->
+            ArStepStar V val e₁ e3 := by
     intros h1 h2
     induction h1 with
     | refl e => exact h2
@@ -184,34 +184,34 @@ theorem eval_completeness (e: ArExpr V) : ArStepStar V val e (ArExpr.Const (eval
     | Const x =>
         simp [eval]
         exact ArStepStar.refl _ _
-    | Add e1 e2 ih1 ih2 =>
-        -- ih1 : ArStepStar e1 (ArExpr.Const (eval e1))
-        -- ih2 : ArStepStar e2 (ArExpr.Const (eval e2))
+    | Add e₁ e₂ ih1 ih2 =>
+        -- ih1 : ArStepStar e₁ (ArExpr.Const (eval e₁))
+        -- ih2 : ArStepStar e₂ (ArExpr.Const (eval e₂))
         simp [eval]
-        have a := arstepstar_add_left _ _ _ e2 ih1
-        have b := arstepstar_add_right _ (eval V val e1) e2 _ ih2
-        have c := ArStep.addConstConst (val := val) (eval V val e1) (eval V val e2)
-        have d := ArStepStar.trans _ _ _ c (ArStepStar.refl _ (ArExpr.Const (eval V val e1 + eval V val e2)))
+        have a := arstepstar_add_left _ _ _ e₂ ih1
+        have b := arstepstar_add_right _ (eval V val e₁) e₂ _ ih2
+        have c := ArStep.addConstConst (val := val) (eval V val e₁) (eval V val e₂)
+        have d := ArStepStar.trans _ _ _ c (ArStepStar.refl _ (ArExpr.Const (eval V val e₁ + eval V val e₂)))
         have e := chasles_step_star _ a (chasles_step_star _ b d)
         exact e
-    | Sub e1 e2 ih1 ih2 =>
-        -- ih1 : ArStepStar e1 (ArExpr.Const (eval e1))
-        -- ih2 : ArStepStar e2 (ArExpr.Const (eval e2))
+    | Sub e₁ e₂ ih1 ih2 =>
+        -- ih1 : ArStepStar e₁ (ArExpr.Const (eval e₁))
+        -- ih2 : ArStepStar e₂ (ArExpr.Const (eval e₂))
         simp [eval]
-        have a := arstepstar_sub_left _ _ _ e2 ih1
-        have b := arstepstar_sub_right _ (eval V val e1) e2 _ ih2
-        have c := ArStep.subConstConst (val := val) (eval V val e1) (eval V val e2)
-        have d := ArStepStar.trans _ _ _ c (ArStepStar.refl _ (ArExpr.Const  (eval V val e1 - eval V val e2)))
+        have a := arstepstar_sub_left _ _ _ e₂ ih1
+        have b := arstepstar_sub_right _ (eval V val e₁) e₂ _ ih2
+        have c := ArStep.subConstConst (val := val) (eval V val e₁) (eval V val e₂)
+        have d := ArStepStar.trans _ _ _ c (ArStepStar.refl _ (ArExpr.Const  (eval V val e₁ - eval V val e₂)))
         have e := chasles_step_star _ a (chasles_step_star _ b d)
         exact e
-    | Mul e1 e2 ih1 ih2 =>
-        -- ih1 : ArStepStar e1 (ArExpr.Const (eval e1))
-        -- ih2 : ArStepStar e2 (ArExpr.Const (eval e2))
+    | Mul e₁ e₂ ih1 ih2 =>
+        -- ih1 : ArStepStar e₁ (ArExpr.Const (eval e₁))
+        -- ih2 : ArStepStar e₂ (ArExpr.Const (eval e₂))
         simp [eval]
-        have a := arstepstar_mul_left _ _ _ e2 ih1
-        have b := arstepstar_mul_right _ (eval V val e1) e2 _ ih2
-        have c := ArStep.mulConstConst (val := val) (eval V val e1) (eval V val e2)
-        have d := ArStepStar.trans _ _ _ c (ArStepStar.refl _ (ArExpr.Const (eval  V val e1 * eval V val e2)))
+        have a := arstepstar_mul_left _ _ _ e₂ ih1
+        have b := arstepstar_mul_right _ (eval V val e₁) e₂ _ ih2
+        have c := ArStep.mulConstConst (val := val) (eval V val e₁) (eval V val e₂)
+        have d := ArStepStar.trans _ _ _ c (ArStepStar.refl _ (ArExpr.Const (eval  V val e₁ * eval V val e₂)))
         have e := chasles_step_star _ a (chasles_step_star _ b d)
         exact e
     | Var var =>
@@ -241,3 +241,74 @@ def eval_bool (val: V -> Int) (e: BoolExpr V): Bool :=
     | BoolExpr.Not e => not (eval_bool val e)
     | BoolExpr.And l r => if eval_bool val l then eval_bool val r else false
     | BoolExpr.Or l r => if eval_bool val l then true else eval_bool val r
+
+inductive BoolStep: (val: V -> Int) -> (BoolExpr V) -> (BoolExpr V) -> Prop where
+    | notFalseIsTrue: BoolStep val
+        (BoolExpr.Not BoolExpr.False)
+        BoolExpr.True
+    | notTrueIsFalse : BoolStep val
+        (BoolExpr.Not BoolExpr.True)
+         BoolExpr.False
+    | andLeftTrue (e: BoolExpr V): BoolStep val
+        (BoolExpr.And BoolExpr.True e)
+        e
+    | andLeftFalse (e: BoolExpr V): BoolStep val
+        (BoolExpr.Or BoolExpr.False e)
+        e
+    | andLeftShortCircuit e : BoolStep val
+        (BoolExpr.And BoolExpr.False e)
+        BoolExpr.False
+    | orLeftShortCircuit e : BoolStep val
+        (BoolExpr.Or BoolExpr.True e)
+        BoolExpr.True
+    | lessConstConst n₁ n₂ : BoolStep val
+        (BoolExpr.Less (ArExpr.Const n₁) (ArExpr.Const n₂))
+        (if n₁ < n₂ then BoolExpr.True else BoolExpr.False)
+    | eqConstConst n₁ n₂ : BoolStep val
+        (BoolExpr.Eq (ArExpr.Const n₁) (ArExpr.Const n₂))
+        (if n₁ == n₂ then BoolExpr.True else BoolExpr.False)
+    | lessArStepLeft (e₁ e₁' e₂: ArExpr V):
+        ArStep V val e₁ e₁' ->
+            BoolStep val
+                (BoolExpr.Less e₁ e₂)
+                (BoolExpr.Less e₁' e₂)
+    | eqArStepLeft (e₁ e₁' e₂: ArExpr V):
+        ArStep V val e₁ e₁' ->
+            BoolStep val
+                (BoolExpr.Eq e₁ e₂)
+                (BoolExpr.Eq e₁' e₂)
+     | lessArStepRight (e₁ e₂ e₂': ArExpr V):
+        ArStep V val e₂ e₂' ->
+            BoolStep val
+                (BoolExpr.Less e₁ e₂)
+                (BoolExpr.Less e₁ e₂')
+    | eqArStepRight (e₁ e₂ e₂': ArExpr V):
+        ArStep V val e₂ e₂' ->
+            BoolStep val
+                (BoolExpr.Eq e₁ e₂)
+                (BoolExpr.Eq e₁ e₂')
+    | orStepLeft (e₁ e₁' e₂: BoolExpr V):
+        BoolStep val e₁ e₁' ->
+            BoolStep val
+                (BoolExpr.Or e₁ e₂)
+                (BoolExpr.Or e₁' e₂)
+    | andStepLeft (e₁ e₁' e₂: BoolExpr V):
+        BoolStep val e₁ e₁' ->
+            BoolStep val
+                (BoolExpr.And e₁ e₂)
+                (BoolExpr.And e₁' e₂)
+
+    | orStepRight (e₁ e₂ e₂': BoolExpr V):
+        BoolStep val e₂ e₂' ->
+            BoolStep val
+                (BoolExpr.Or e₁ e₂)
+                (BoolExpr.Or e₁ e₂')
+    | andStepRight (e₁ e₂ e₂': BoolExpr V):
+        BoolStep val e₂ e₂' ->
+            BoolStep val
+                (BoolExpr.And e₁ e₂)
+                (BoolExpr.And e₁ e₂')
+    | notStep (e e' : BoolExpr V):
+        BoolStep val e e' -> BoolStep val
+            (BoolExpr.Not e)
+            (BoolExpr.Not e')
